Progress on memory related cheats

pancake/proofs/ffiTimeScript.sml
@@ -18,29 +18,51 @@ Type pan_state = ``:('a, time_input) panSem$state``
 Overload k2mw = “multiword$k2mw”
 
 
+Definition get_bytes_def:
+  get_bytes (:'a) n =
+  let m  = dimindex (:'a) DIV 8;
+      as = GENLIST (λm. (n2w m): 'a word) m;
+      w  = (n2w n):'a word
+  in
+    MAP (λa. get_byte a w F) as
+End
+
+
+Definition ntime_input_def:
+  ntime_input (:'a) (f:num -> num # bool) =
+  let
+    t = FST (f 0);
+    b = if SND (f 0) then 0 else 1
+  in
+    get_bytes (:'a) t ++
+    get_bytes (:'a) b
+End
+
 Definition next_ffi_def:
   next_ffi (f:num -> (num # bool)) =
     λn. f (n+1)
 End
 
 
+Definition build_ffi_def:
+  build_ffi (:'a) (seq:time_input) io =
+     <| oracle    :=
+        (λs f conf bytes.
+          if s = "get_ffi"
+          then Oracle_return (next_ffi f) (ntime_input (:'a) f)
+          else Oracle_final FFI_failed)
+      ; ffi_state := seq
+      ; io_events := io|> : time_input_ffi
+End
+
+
+(*
 Definition ntime_input_def:
   ntime_input (f:num -> num # bool) n =
     ((k2mw (n-1) (FST (f 0))):word8 list) ++
     [if SND (f 0) then 0w else 1w]
 End
-
-
-Definition build_ffi_def:
-  build_ffi (seq:time_input) io =
-     <| oracle    :=
-        (λs f conf bytes.
-          if s = "get_ffi"
-          then Oracle_return (next_ffi f) (ntime_input f (LENGTH bytes))
-          else Oracle_final FFI_failed)
-      ; ffi_state := seq
-      ; io_events := io|> : time_input_ffi
-End
+*)
 
 (*
 [IO_event "get_ffi" []
